jwnregjbwrgwrb

Games/games/Chomp_work.lean
@@ -66,6 +66,12 @@ lemma Chomp_state_sub' (ini : Finset (ℕ × ℕ)) (l L :  List (ℕ × ℕ)) :
     apply xdef.2
     exact List.mem_append_right l ql
 
+lemma Chomp_state_cons (ini : Finset (ℕ × ℕ)) (l :  List (ℕ × ℕ)) (x : ℕ × ℕ) :
+  Chomp_state ini (x :: l) ⊆ Chomp_state ini l :=
+  by
+  rw [List.cons_eq_singleton_append]
+  apply Chomp_state_sub'
+
 
 def Chomp_init (height length : ℕ) := (Finset.range (length+1)) ×ˢ (Finset.range (height+1))
 
@@ -100,7 +106,7 @@ lemma Chomp_state_blind (ini : Finset (ℕ × ℕ)) (hist prehist : List (ℕ ×
 
 inductive Chomp_law (ini : Finset (ℕ × ℕ)) : List (ℕ × ℕ) → ℕ × ℕ →  Prop where
 | nil (act : ℕ × ℕ) : act ∈ ini →  act ≠ (0,0) → Chomp_law ini [] act
-| cons (act : ℕ × ℕ) (l : List (ℕ × ℕ)) (x : ℕ × ℕ) : Chomp_law ini l act →  act ∈ Chomp_state ini (x :: l) →  act ≠ (0,0) → Chomp_law ini (x :: l) act
+| cons (act : ℕ × ℕ) (l : List (ℕ × ℕ)) (x : ℕ × ℕ) : Chomp_law ini l x →  act ∈ Chomp_state ini (x :: l) →  act ≠ (0,0) → Chomp_law ini (x :: l) act
 
 
 def preChomp (height length : ℕ) : Symm_Game_World (Finset (ℕ × ℕ)) (ℕ × ℕ) where
@@ -202,13 +208,11 @@ lemma Chomp_law_state_mem (ini : Finset (ℕ × ℕ) ) (hist : List (ℕ × ℕ)
     exact c
 
 
--- lemma Chomp_law_sub (ini : Finset (ℕ × ℕ) ) (l L : List (ℕ × ℕ)) (act : ℕ × ℕ) (leg : Chomp_law ini (l ++ L) act) :
---   Chomp_law ini L act :=
---   by
---   refine' ⟨leg.act_mem, _ , leg.nz_act⟩
---   intro q qdef
---   apply leg.nd
---   exact List.mem_append_right l qdef
+lemma Chomp_law_ini_mem (ini : Finset (ℕ × ℕ) ) (hist : List (ℕ × ℕ)) (act : ℕ × ℕ) (leg : Chomp_law ini hist act) :
+  act ∈ ini  :=
+  by
+  apply Chomp_state_sub_ini _ hist
+  apply Chomp_law_state_mem _ _ _ leg
 
 
 
@@ -220,7 +224,7 @@ lemma Chomp_law_act_nz (ini : Finset (ℕ × ℕ) ) (hist : List (ℕ × ℕ)) (
     rename_i _ a
     exact a
   · cases' leg
-    rename_i a _ _
+    rename_i _ a _
     exact a
 
 
@@ -244,6 +248,62 @@ lemma Chomp_hist_no_zero_of_Hist_legal (height length : ℕ) (ini : Finset (ℕ 
                     apply Chomp_law_act_nz _ _ _ now}
     · exact ih sofar
 
+
+lemma Chomp_state_empty_hist (ini : Finset ( ℕ × ℕ)) : Chomp_state ini [] = ini :=
+  by
+  dsimp [Chomp_state]
+  rw [Finset.filter_eq_self]
+  intro _ _ _ no
+  contradiction
+
+lemma Chomp_hist_legal  (ini : Finset (ℕ × ℕ) ) (prehist hist : List (ℕ × ℕ)) (act : ℕ × ℕ)
+  --(main : Chomp_law ini prehist)
+  : Chomp_law ini (hist ++ prehist) act ↔  Chomp_law (Chomp_state ini prehist) (hist) act :=
+  by
+  induction' hist with x l ih
+  · constructor
+    · intro main
+      cases' main
+      · rename_i h1 h2
+        apply Chomp_law.nil _ _ h2
+        rw [Chomp_state_empty_hist]
+        exact h1
+      · rename_i l x h1 h2 h3
+        apply Chomp_law.nil _ h2 h3
+    · intro main
+      cases' main
+      rename_i h1 h2
+      revert act
+      induction' prehist with x l ih
+      · intro act h1 h2
+        apply Chomp_law.nil
+        · rwa [Chomp_state_empty_hist] at h1
+        · exact h2
+      · intro act h1 h2
+        dsimp
+        apply Chomp_law.cons _ _ _ _ h1 h2
+        apply ih
+        -- restore prehist ≠ [] (?) and Hist_leg to get this ??
+        exact Chomp_state_cons _ _ _ h1
+  · constructor
+    · intro main
+      rw [List.cons_append] at main
+      cases' main
+      rename_i h1 h2 h3
+      apply Chomp_law.cons  _ _ _ (ih.mp h2) _ h1
+      rw [Chomp_state_blind]
+      rw [List.cons_append]
+      exact h3
+    · intro main
+      rw [List.cons_append]
+      cases' main
+      rename_i h1 h2 h3
+      apply Chomp_law.cons _ _ _ (ih.mpr h2) _ h1
+      rw [Chomp_state_blind] at h3
+      rw [List.cons_append] at h3
+      exact h3
+
+
 #exit
 
 lemma preChomp_law_careless (height length : ℕ) :
@@ -265,19 +325,7 @@ lemma preChomp_law_careless (height length : ℕ) :
           by_cases q3 : Chomp_state ini (List.tail prehist) ≠ {(0, 0)}
           · rw [if_pos q3] at *
             split_ifs
-            all_goals { constructor
-                        · dsimp [Chomp_state]
-                          rw [Finset.mem_filter]
-                          constructor
-                          · exact c.act_mem
-                          · intro e eh
-                            apply (c.nd e (List.mem_append_right hist eh)).1
-                        · intro e eh
-                          refine' ⟨ (c.nd e (by exact List.mem_append_left prehist eh)).1, _ ⟩
-                          have := (c.nd e (by exact List.mem_append_left prehist eh)).2
-
-                        · apply c.nz_act
-            }
+            all_goals { exact (Chomp_hist_legal _ _ _ _).mp c}
           · rw [if_neg q3] at *
             exfalso
             have : Chomp_state {(0, 0)} hist ⊂ {(0, 0)} :=
@@ -291,14 +339,13 @@ lemma preChomp_law_careless (height length : ℕ) :
             rw [iff_not_comm] at that
             rw [this] at that
             simp only [Finset.not_mem_empty, not_false_eq_true, iff_true] at that
-            have thut := c.nd (0,0) (by exact List.mem_append_left prehist that)
-            dsimp [nondomi, domi] at thut
-            apply thut
-            simp only [zero_le, and_self]
+            have actually := Chomp_law_state_mem _ _ _ c
+            rw [Chomp_state_hist_zero _ (hist ++ prehist) (by exact List.mem_append_left prehist that)] at actually
+            contradiction
         · dsimp [preChomp] at *
           rw [if_neg q2]
           split_ifs
-          all_goals apply c.nz_act
+          all_goals apply (Chomp_law_act_nz _ _ _ c)
       · rw [if_neg q1] at c
         by_cases q2 : Chomp_state (Symm_Game_World.transition (preChomp height length) ini (List.tail prehist) (List.head prehist pHne)) (hist) ≠ {(0,0)}
         · dsimp [preChomp] at *
@@ -349,18 +396,7 @@ lemma preChomp_law_careless (height length : ℕ) :
           by_cases q3 : Chomp_state (Chomp_state ini prehist) hist ≠ {(0, 0)}
           · rw [if_pos q3] at c
             rw [if_pos] at c
-            constructor
-            · apply Chomp_state_sub_ini
-              apply c.act_mem
-            · have := c.act_mem
-              dsimp [Chomp_state] at this
-              rw [Finset.mem_filter] at this
-              intro e eh
-              rw [List.mem_append] at eh
-              · cases' eh with k k
-                · exact c.nd e k
-                · exact this.2 e k
-            · exact c.nz_act
+            · exact (Chomp_hist_legal _ _ _ _).mpr c
             · rw [Chomp_state_has_zero_iff_hist_has_zero ini fix.1 prehist]
               exact ⟨Chomp_hist_no_zero_of_Hist_legal height length ini fix.1 prehist pHl, fix.2⟩
           · rw [if_neg q3] at c
@@ -372,8 +408,8 @@ lemma preChomp_law_careless (height length : ℕ) :
           by_cases q3 : Chomp_state {(0, 0)} hist ≠ {(0, 0)}
           · rw [if_pos q3, if_pos ⟨ (by apply Finset.mem_singleton_self) , fix.2⟩ ] at c
             exfalso
-            apply c.nz_act
-            have := c.act_mem
+            apply (Chomp_law_act_nz _ _ _ c)
+            have := Chomp_law_ini_mem _ _ _ c
             rwa [Finset.mem_singleton] at this
           · rw [if_neg q3] at c
             rw [not_not] at q3 q2
@@ -427,12 +463,12 @@ lemma preChomp_law_careless (height length : ℕ) :
       · rw [if_neg q1]
         split_ifs at c
         · exact c
-        · apply c.nz_act
+        · apply (Chomp_law_act_nz _ _ _ c)
         · rename_i no
           push_neg at no
           exact False.elim (fix.2 (no (by apply Finset.mem_singleton_self)))
         · exact c
-        · apply c.nz_act
+        · apply (Chomp_law_act_nz _ _ _ c)
         · exfalso
           rename_i no
           apply no
@@ -453,7 +489,7 @@ lemma preChomp_law_careless (height length : ℕ) :
     · rename_i a b c
       exact False.elim (by apply fix ; constructor ; apply Chomp_state_sub_ini ; apply b.1 ; apply b.2)
 
-#exit
+
 
 
 lemma preChomp_tranistion_careless (height length : ℕ) :
@@ -613,7 +649,7 @@ lemma preChomp_coherent (height length : ℕ)  : (preChomp height length).cohere
             specialize f_leg t tu
             by_cases split_ifs_is_wierd : ¬Chomp_state (Chomp_init height length) (History_on_turn (Chomp_init height length) f_strat s_strat t) = {(0, 0)}
             · rw [if_pos ⟨(Chomp_init_has_zero _ _), (by rw [← Chomp_state_has_zero_iff_hist_has_zero (Chomp_init height length) (Chomp_init_has_zero _ _ ), k] ; apply Finset.mem_singleton_self )⟩ , if_pos (split_ifs_is_wierd)] at f_leg
-              exact f_leg.nz_act
+              exact (Chomp_law_act_nz _ _ _ f_leg)
             · rw [if_pos ⟨(Chomp_init_has_zero _ _ ), (by rw [← Chomp_state_has_zero_iff_hist_has_zero (Chomp_init height length) (Chomp_init_has_zero _ _ ), k] ; apply Finset.mem_singleton_self )⟩, if_neg (split_ifs_is_wierd)] at f_leg
               exact f_leg
           apply Chomp_state_zero_act_non_zero
@@ -625,7 +661,7 @@ lemma preChomp_coherent (height length : ℕ)  : (preChomp height length).cohere
             specialize s_leg t tu
             by_cases split_ifs_is_wierd : ¬Chomp_state (Chomp_init height length) (History_on_turn (Chomp_init height length) f_strat s_strat t) = {(0, 0)}
             · rw [if_pos ⟨(Chomp_init_has_zero _ _ ), (by rw [← Chomp_state_has_zero_iff_hist_has_zero (Chomp_init height length) (Chomp_init_has_zero _ _ ), k] ; apply Finset.mem_singleton_self )⟩, if_pos (split_ifs_is_wierd)] at s_leg
-              exact s_leg.nz_act
+              exact (Chomp_law_act_nz _ _ _ s_leg)
             · rw [if_pos ⟨(Chomp_init_has_zero _ _ ), (by rw [← Chomp_state_has_zero_iff_hist_has_zero (Chomp_init height length) (Chomp_init_has_zero _ _ ), k] ; apply Finset.mem_singleton_self )⟩, if_neg (split_ifs_is_wierd)] at s_leg
               exact s_leg
           apply Chomp_state_zero_act_non_zero
@@ -654,7 +690,7 @@ lemma preChomp_coherent (height length : ℕ)  : (preChomp height length).cohere
             specialize f_leg t tu
             by_cases split_ifs_is_wierd : ¬Chomp_state (Chomp_init height length) (History_on_turn (Chomp_init height length) f_strat s_strat t) = {(0, 0)}
             · rw [if_pos ⟨(Chomp_init_has_zero _ _ ), (by rw [← Chomp_state_has_zero_iff_hist_has_zero (Chomp_init height length) (Chomp_init_has_zero _ _ ), k] ; apply Finset.mem_singleton_self )⟩, if_pos (split_ifs_is_wierd)] at f_leg
-              exact f_leg.nz_act
+              exact (Chomp_law_act_nz _ _ _ f_leg)
             · rw [if_pos ⟨(Chomp_init_has_zero _ _ ), (by rw [← Chomp_state_has_zero_iff_hist_has_zero (Chomp_init height length) (Chomp_init_has_zero _ _ ), k] ; apply Finset.mem_singleton_self )⟩, if_neg (split_ifs_is_wierd)] at f_leg
               exact f_leg
           apply Chomp_state_zero_act_non_zero
@@ -666,7 +702,7 @@ lemma preChomp_coherent (height length : ℕ)  : (preChomp height length).cohere
             specialize s_leg t tu
             by_cases split_ifs_is_wierd : ¬Chomp_state (Chomp_init height length) (History_on_turn (Chomp_init height length) f_strat s_strat t) = {(0, 0)}
             · rw [if_pos ⟨(Chomp_init_has_zero _ _ ), (by rw [← Chomp_state_has_zero_iff_hist_has_zero (Chomp_init height length) (Chomp_init_has_zero _ _ ), k] ; apply Finset.mem_singleton_self )⟩, if_pos (split_ifs_is_wierd)] at s_leg
-              exact s_leg.nz_act
+              exact (Chomp_law_act_nz _ _ _ s_leg)
             · rw [if_pos ⟨(Chomp_init_has_zero _ _ ), (by rw [← Chomp_state_has_zero_iff_hist_has_zero (Chomp_init height length) (Chomp_init_has_zero _ _ ), k] ; apply Finset.mem_singleton_self )⟩, if_neg (split_ifs_is_wierd)] at s_leg
               exact s_leg
           apply Chomp_state_zero_act_non_zero
@@ -676,6 +712,7 @@ lemma preChomp_coherent (height length : ℕ)  : (preChomp height length).cohere
       · dsimp [History_on_turn]
         rw [if_pos (by rw [Turn_fst_not_step] ; exact q1)]
         exact main
+
 
 
 lemma preChomp_playable (height length : ℕ) : (preChomp height length).playable :=
@@ -712,17 +749,30 @@ lemma preChomp_playable (height length : ℕ) : (preChomp height length).playabl
           · exact con.2.symm
       obtain ⟨act, act_mem, act_nz⟩ := this
       use act
-      constructor
-      · exact (Chomp_state_sub_ini _ _) act_mem
-      · dsimp [Chomp_state] at act_mem
-        rw [Finset.mem_filter] at act_mem
-        exact act_mem.2
-      · exact act_nz
+      induction' hist with x l ih
+      · apply Chomp_law.nil _ _ act_nz
+        rw [Chomp_state_empty_hist] at act_mem
+        exact act_mem
+      · apply Chomp_law.cons _ _ _ _ act_mem act_nz
+        rename_i h
+        apply ih
+        · contrapose! q
+          apply Chomp_state_zero_act_non_zero _ h.1 _ _ q
+          intro con
+          rw [con] at h
+          apply h.2
+          exact List.mem_cons_self (0, 0) l
+        · refine' ⟨ h.1, _ ⟩
+          intro con
+          apply h.2
+          exact List.mem_cons_of_mem x con
+        · apply Chomp_state_cons _ _ _ act_mem
     · use (0,0)
   · simp_rw [if_neg q]
     use (1,0)
     split_ifs
     · decide
+
 
 
 def Chomp (height length : ℕ) : zSymm_Game_World (Finset (ℕ × ℕ)) (ℕ × ℕ) where
@@ -781,15 +831,15 @@ lemma preChomp_law_prop_transition (height length : ℕ) (h : height ≠ 0 ∨ l
             contrapose! ca
             constructor
             · apply le_trans _ ca.1
-              have := leg.act_mem
-              dsimp [Chomp_init] at this
-              rw [Finset.mem_product, Finset.mem_range, Nat.lt_add_one_iff] at this
-              exact this.1
+              have := (Chomp_law_state_mem _ _ _ leg)
+              dsimp [Chomp_state, Chomp_init] at this
+              simp_rw [Finset.mem_filter, Finset.mem_product, Finset.mem_range, Nat.lt_add_one_iff] at this
+              exact this.1.1
             · apply le_trans _ ca.2
-              have := leg.act_mem
-              dsimp [Chomp_init] at this
-              simp_rw [Finset.mem_product, Finset.mem_range, Nat.lt_add_one_iff] at this
-              exact this.2
+              have := (Chomp_law_state_mem _ _ _ leg)
+              dsimp [Chomp_state, Chomp_init] at this
+              simp_rw [Finset.mem_filter, Finset.mem_product, Finset.mem_range, Nat.lt_add_one_iff] at this
+              exact this.1.2
         · intro ca
           intro q qdef
           exact ca _ (Or.inl (qdef))
@@ -818,7 +868,7 @@ lemma preChomp_law_prop_transition (height length : ℕ) (h : height ≠ 0 ∨ l
           · dsimp [nondomi, domi]
             intro con
             simp_rw [Nat.le_zero] at con
-            apply leg.nz_act
+            apply (Chomp_law_act_nz _ _ _ leg)
             rw [← qdef]
             ext
             · exact con.1
@@ -850,7 +900,6 @@ lemma preChomp_law_prop_transition (height length : ℕ) (h : height ≠ 0 ∨ l
     rw [Chomp_state_hist_zero _ (act ::(hist ++ [(length, height)])) (List.mem_cons_of_mem _ (List.mem_append_left _ q1))]
 
 
-
 lemma preChomp_law_prop_law (height length : ℕ) (h : height ≠ 0 ∨ length ≠ 0) (act : ℕ × ℕ) (hist : List (ℕ × ℕ)) (hh : hist ≠ [])
   (leg : Symm_Game_World.law (Chomp height length).toSymm_Game_World (Chomp height length).toSymm_Game_World.init_game_state hist act) :
   Symm_Game_World.law (Chomp height length).toSymm_Game_World (Chomp height length).toSymm_Game_World.init_game_state
@@ -872,28 +921,18 @@ lemma preChomp_law_prop_law (height length : ℕ) (h : height ≠ 0 ∨ length �
       · rw [if_pos q1] at leg
         by_cases q2 : ¬Chomp_state (Chomp_init height length) (hist ++ [(length, height)]) = {(0, 0)}
         · rw [if_pos q2]
-          constructor
-          · exact leg.act_mem
-          · intro q qdef
-            rw [List.mem_append] at qdef
-            cases' qdef with qdef qdef
-            · exact leg.nd _ qdef
-            · rw [List.mem_singleton] at qdef
-              rw [qdef]
-              dsimp [nondomi, domi]
-              induction' hist with x hist ih
-              · contradiction
-              · have leg1 := leg.act_mem
-                dsimp [Chomp_init] at leg1
-                simp_rw [Finset.mem_product, Finset.mem_range, Nat.lt_add_one_iff] at leg1
-                have leg2 := leg.nd x (List.mem_cons_self x hist)
-
-          · exact leg.nz_act
+          induction' hist with x l ih
+          · contradiction
+          · cases' leg
+            rename_i h1 h2 h3
+            rw [List.cons_append]
+            apply Chomp_law.cons
         · rw [if_neg q2]
-          exact leg.nz_act
+          exact (Chomp_law_act_nz _ _ _ leg)
       · rw [if_neg q1] at leg
 
 
+#exit
 
 
 
